# Derivative Rules

## Essential
<u>**General**</u>
$$
f(x)=k \quad\longrightarrow\quad f'(x)=0  
$$

<pre></pre>
$$
f(x)=x^n \quad\longrightarrow\quad f'(x)=nx^{n-1}
$$

<pre></pre>
$$
y=f(x)\pm g(x) \quad\longrightarrow\quad y'=f'(x)\pm g'(x) 
$$

<pre></pre>
$$
y=\left[f(x)\right]^n \quad\longrightarrow\quad y'=n\left[f(x)\right]^{n-1}f'(x) 
$$

<pre></pre>
$$
y=f(x)g(x) \quad\longrightarrow\quad y'=f(x)g'(x)+g(x)f'(x)
$$

<pre></pre>
$$
y=\frac{f(x)}{g(x)} \quad\longrightarrow\quad y'=\frac{g(x)f'(x)-f(x)g'(x)}{\left[g(x)\right]^2}  
$$


<pre>

</pre>
<u>**Trig**</u>

$$
y=\sin(x) \quad\longrightarrow\quad y'=\cos(x)x'
$$

<pre></pre>
$$
y=\cos(x) \quad\longrightarrow\quad y'=-\sin(x)x'
$$

<pre></pre>
$$
y=\tan(x) \quad\longrightarrow\quad y'=\sec^2(x)x' 
$$

<pre>

</pre>
<u>**Exponential**</u>
$$
y=e^x \quad\longrightarrow\quad y'=e^xx'  
$$

<pre></pre>
$$
y=b^x \quad\longrightarrow\quad y'=ln(b)b^xx'  
$$


<pre>

</pre>
<u>**Log**</u>
$$
y=ln(x) \quad\longrightarrow\quad y'=\frac{x'}{x}  
$$

<pre></pre>
$$
y=log_bx \quad\longrightarrow\quad y'=\frac{x'}{ln(b)x}  
$$

## Implied
$$
f(x)=mx \quad\longrightarrow\quad f'(x)=m  
$$

<pre></pre>
$$
f(x)=mx+b \quad\longrightarrow\quad f'(x)=m 
$$
<pre>

</pre>
## Derivative rules with values
Follow all the normla derivative rules, but substitute in values when doing the derivative

>Ex: If $f(x) = 3$, $f'(x) = -2$, $g(x) = 5$, and $g'(x) = 7$, find $y'$
><pre></pre>
>I) $y = f(x)g(x)$
>$y' = 3(7) + 5(-2)$
>$y' = 11$
><pre></pre>
>II) $y = \frac{f(x)}{g(x)}$
>$y' = \frac{5(-2)-(3)(7)}{5^2}$
>$y' = \frac{-31}{25}$
><pre></pre>
>III) $y =[f(x)]^2$
>$y' = 2(3)(-2)$
>$y' = -12$