# Simplifying Derivatives
Follows the same general format:
1. Factor out any greatest common factors (GCF)
2. Cancel any factors with the denominator
3. Expand the remaining factors
4. Collect like terms

>Ex: $y = (x^4-5x+3)(x^3-6)$
>$$
\begin{align}
>y' &= (x^2-5x+3)(3x^2) + (x^3-6)(2x-5) \\
>y' &= 3x^4 - 15x^3 +9x^2 +2x^4 -5x^3 -12x +30 \\
>y' &= 5x^4 -20x^3 +9x^2 -12x +30
\end{align}
>$$

>Ex: $y = (x^2 - 4)^6(3x^2 +2)$
>$$
\begin{align}
>y' &= (x^2-4)^6(6x)+ (3x^2+2)(6)(x^2-4)^5(2x) \\
>y' &= 6x(x^2-4)^5[(x^2-4)+2(3x^2+2)] \\
>y' &= 6x(x^2-4)^5(7x^2)
\end{align}
>$$

>Ex: $y = \frac{4x}{(2x^3 +3)^5}$
>$$
\begin{align}
>y' &= \frac{(2x^3 +3)^5(4)-(4x)(5)(2x^3 +3)^4(6x^2)}{(2x^3 +3)^{10}} \\
>y' &= \frac{4(2x^3 +3)^4[2x^3+3 - (x)(5)(6x^2)]}{(2x^3 +3)^{10}} \\
>y' &= \frac{4(-28x^3+3)}{(2x^3 +3)^6} \\
\end{align}
>$$
